WIP: multi port max_op

dataplane/Examples/Max_top.thy
@@ -2,63 +2,64 @@ theory Max_top
 
 imports
   "../Timely_Infrastructure"
-  "HOL-Library.Finite_Map"
   Input_top
 begin 
+
+
 
 definition "maxs buf = [(n, c) \<leftarrow> buf. n = Max (set (map fst ((filter (\<lambda> (n' :: nat, c'). time c = time c') buf))))]"
 
 (* FIXME: move me *)
 abbreviation "choice5 op1 op2 op3 op4 op5 \<equiv> choice3 (choice2 op1 op2) (choice2 op3 op4) op5"
 
-find_consts "  _ \<Rightarrow>(_ \<times> _) list \<Rightarrow> _ \<Rightarrow> _" 
+find_consts "_ + _ \<Rightarrow> _" name: "is_"
+
+find_theorems is_Inl
 
 
 abbreviation "mint_cap os p t \<equiv> os\<lparr> inter := inter os @ [(p, t, 1)] \<rparr>"
 
-
 corec max_top' where
   "max_top' os buf caps = choice5
    (Read None (\<lambda> st. if is_Inl st \<and> is_Inr (projl st) then max_top' (os\<lparr> front := projr (projl st) \<rparr>) buf caps else \<oslash>))
-   (Choice (cimage (\<lambda> p.
-    let below_caps = [cap \<leftarrow> caps. less_than_frontier (front os p) (time cap)] in
-    let above_caps = [cap \<leftarrow> caps. \<not> less_than_frontier (front os p) (time cap)] in
-    let batches = map (\<lambda> cap. (Max (buf cap), cap)) below_caps in
+   (let below_caps = [cap \<leftarrow> caps. less_than_frontier (front os 0) (time cap)] in
+    let above_caps = [cap \<leftarrow> caps. \<not> less_than_frontier (front os 0) (time cap)] in
+    let batches = map (\<lambda> cap. (Max (set (buf cap)), cap)) below_caps in
     let os' = foldl (\<lambda> os (m, cap). produce os cap [m]) os batches in
     let os'' = foldl drop_cap os' below_caps in
-    let buf' = foldl (\<lambda> s cap. buf(cap := {})) buf below_caps in
-    Silent (max_top' os'' buf' above_caps)) c\<UU>))
-   (Choice (cimage (\<lambda> p. 
-    Read (Some p)
-    (\<lambda> x. if isl x then \<oslash> else
+    let buf' = foldl (\<lambda> s cap. buf(cap := [])) buf below_caps in
+    Silent (max_top' os'' buf' above_caps))
+   (Read (Some 0)
+    (\<lambda> x. if is_Inl x then \<oslash> else
      let (n, t) = projr x in
-     let (caps', os') = (if Cap t p \<in> set caps then (caps, os) else (caps @ [Cap t p], mint_cap os p t)) in
-     let buf' = buf((Cap t p) := insert n (buf (Cap t p))) in
-     max_top' os' buf' caps')) c\<UU>))
-    (Choice (cimage (\<lambda> p. (case outpu os p of
-         x # xs \<Rightarrow> send_output (max_top' (os\<lparr> outpu := (outpu os)(p := xs ) \<rparr>) buf caps) p x)) 
-    (cfilter (\<lambda> p. outpu os p \<noteq> []) c\<UU>)))
+     let (caps', os') = (if Cap t 0 \<in> set caps then (caps, os) else (caps @ [Cap t 0], mint_cap os 0 t)) in
+     let buf' = buf((Cap t 0) := n # (buf (Cap t 0))) in
+     max_top' os' buf' caps'))
+    ((case outpu os 0 of
+         [] \<Rightarrow> Silent (max_top' os buf caps)
+       |  x # xs \<Rightarrow> send_output (max_top' (os\<lparr> outpu := (outpu os)(0 := xs ) \<rparr>) buf caps) 0 x))
     (let (os', st) = obtain_progress os in
      send_progress (max_top' os' buf caps) st)"
 
 lemma step_max'_top_elim:
   assumes "step io (max_top' os buf caps) op"
   obtains
-    st where "io = Inp None st" "is_Inl st" "is_Inr (projl st)" "op = max_top' (os\<lparr> front := projr (projl st) \<rparr>) buf caps"
-  | st where "io = Inp None st" "\<not> is_Inl st \<or> \<not> is_Inr (projl st)" "op = \<oslash>"
-  | p above_caps below_caps batches os' os'' buf' where "io = Tau" "below_caps = [cap \<leftarrow> caps. less_than_frontier (front os p) (time cap)]"
-    "above_caps = [cap \<leftarrow> caps. \<not> less_than_frontier (front os p) (time cap)]"
-    "batches = map (\<lambda> cap. (Max (buf cap), cap)) below_caps"
+    st where "io = Inp None st" "\<not> is_Inl st \<or> (is_Inl st \<and> \<not> is_Inr (projl st))" "op = \<oslash>" 
+  | st where "io = Inp None st" "is_Inl st" "is_Inr (projl st)" "op = max_top' (os\<lparr> front := projr (projl st) \<rparr>) buf caps" 
+  | above_caps below_caps batches os' os'' buf' where "io = Tau" "below_caps = [cap \<leftarrow> caps. less_than_frontier (front os 0) (time cap)]"
+    "above_caps = [cap \<leftarrow> caps. \<not> less_than_frontier (front os 0) (time cap)]"
+    "batches = map (\<lambda> cap. (Max (set (buf cap)), cap)) below_caps"
     "os' = foldl (\<lambda> os (m, cap). produce os cap [m]) os batches"
     "os'' = foldl drop_cap os' below_caps"
-    "buf' = foldl (\<lambda> s cap. buf(cap := {})) buf below_caps"
-    "op = max_top' os'' buf' above_caps" "p \<notin> defaults"
-  | p x where "io = Inp (Some p) x" "isl x" "op = \<oslash>"
-  | p x n t caps' os' buf' where "io = Inp (Some p) x" "\<not> isl x" "(n, t) = projr x"
-    "(caps', os') = (if Cap t p \<in> set caps then (caps, os) else (caps @ [Cap t p], mint_cap os p t))"
-    "buf' = buf((Cap t p) := insert n (buf (Cap t p)))" "op = max_top' os' buf' caps'"
-  | p x xs where "io = Out (Some p) (Inr x)" "outpu os p = x # xs"
-    "op = max_top' (os\<lparr> outpu := (outpu os)(p := xs ) \<rparr>) buf caps" "p \<notin> defaults"
+    "buf' = foldl (\<lambda> s cap. buf(cap := [])) buf below_caps"
+    "op = max_top' os'' buf' above_caps"
+  | x where "io = Inp (Some 0) x" "isl x" "op = \<oslash>"
+  | x n t caps' os' buf' where "io = Inp (Some 0) x" "\<not> isl x" "(n, t) = projr x"
+    "(caps', os') = (if Cap t 0 \<in> set caps then (caps, os) else (caps @ [Cap t 0], mint_cap os 0 t))"
+    "buf' = buf((Cap t 0) := n # (buf (Cap t 0)))" "op = max_top' os' buf' caps'"
+  | "io = Tau" "outpu os 0 = []" "op = max_top' os buf caps"
+  | x xs where "io = Out (Some 0) (Inr x)" "outpu os 0 = x # xs"
+    "op = max_top' (os\<lparr> outpu := (outpu os)(0 := xs ) \<rparr>) buf caps"
   | os' st where "io = Out None (Inl (Inl st))" "obtain_progress os = (os', st)"
     "op = max_top' os' buf caps"
   using assms apply -
@@ -67,19 +68,19 @@ lemma step_max'_top_elim:
   apply (cases io)
   subgoal for p x
     apply simp
-    apply (cases p; simp)
+    apply (cases p; simp; hypsubst_thin)
     subgoal
-      by (auto 0 0 split: if_splits list.splits)
+      by (auto del: disjCI split: if_splits list.splits sum.splits; hypsubst_thin?)
     subgoal
-      by (fastforce split: prod.splits if_splits list.splits)
+      by (cases x; force split: if_splits list.splits sum.splits; hypsubst_thin?)
     done
   subgoal for p x
     apply simp
-    apply (cases p; simp)
+    apply (cases p; simp; hypsubst_thin)
     subgoal
-      by (auto 0 0 split: if_splits list.splits)
+      by (auto del: disjCI split: if_splits list.splits sum.splits; hypsubst_thin?)
     subgoal
-      by (fastforce split: prod.splits if_splits list.splits)
+      by (cases x; force split: if_splits list.splits sum.splits; hypsubst_thin?)
     done
   subgoal
     by (fastforce split: if_splits list.splits)
@@ -100,7 +101,7 @@ corec max_op where
   "max_op n inps = Choice (cimage (\<lambda> p. case ldropWhile ((=) []) (inps p) of
      LCons xs lxs \<Rightarrow> 
      Write 
-     (max_op (n(p := n p + the_enat (llength (ltakeWhile ((=) []) (inps p))))) (inps (p := lxs)))
+     (max_op (n(p := n p + 1 + the_enat (llength (ltakeWhile ((=) []) (inps p))))) (inps (p := lxs)))
        p (Max (set xs), n p + the_enat (llength (ltakeWhile ((=) []) (inps p)))))
      (cfilter (\<lambda> p. ldropWhile ((=) []) (inps p) \<noteq> LNil) c\<UU>))"
 
@@ -108,7 +109,7 @@ corec max_op where
 lemma step_max_op_elim:
   assumes "step io (max_op n inps) op"
   obtains p xs lxs where "io = Out p (Max (set xs), n p + the_enat (llength (ltakeWhile ((=) []) (inps p))))" "ldropWhile ((=) []) (inps p) = LCons xs lxs"
-    "op = max_op (n (p := n p + the_enat (llength (ltakeWhile ((=) []) (inps p))))) (inps(p := lxs))" "p \<notin> defaults"
+    "op = max_op (n (p := n p + 1 + the_enat (llength (ltakeWhile ((=) []) (inps p))))) (inps(p := lxs))" "p \<notin> defaults"
   using assms apply -
   apply atomize_elim
   apply (subst (asm) max_op.code)
@@ -120,7 +121,7 @@ lemma step_max_op_Out_intro[intro]:
    xs \<noteq> [] \<Longrightarrow>
    ys = inps(p := lxs) \<Longrightarrow>
    p \<notin> defaults \<Longrightarrow>
-   step (Out p (Max (set xs), n p)) (max_op n inps) (max_op n ys)"
+   step (Out p (Max (set xs), n p)) (max_op n inps) (max_op (n(p := Suc (n p))) ys)"
   apply (subst max_op.code)
   apply (clarsimp split: llist.splits)
   apply (rule SC)
@@ -135,7 +136,7 @@ lemma step_max_op_Out_intro2[intro]:
   "ldropWhile ((=) []) (inps p) = LCons xs lxs \<Longrightarrow>
    xs \<noteq> [] \<Longrightarrow>
    p \<notin> defaults \<Longrightarrow>
-   step (Out p (Max (set xs), (n p) + the_enat (llength (ltakeWhile ((=) []) (inps p))))) (max_op n inps) (max_op (n (p := n p + the_enat (llength (ltakeWhile ((=) []) (inps p))))) (inps(p := lxs)))"
+   step (Out p (Max (set xs), (n p) + the_enat (llength (ltakeWhile ((=) []) (inps p))))) (max_op n inps) (max_op (n (p := n p + 1 + the_enat (llength (ltakeWhile ((=) []) (inps p))))) (inps(p := lxs)))"
   apply (subst max_op.code)
   apply (rule SC)
    apply (rule cimage_eqI[rotated])
@@ -178,7 +179,7 @@ abbreviation "m_top os buf caps \<equiv>  map_op (case_option (Inl (1 :: 2)) (\<
 
 abbreviation "inp_m_top os1 caps1 inps buf1 os2 buf2 caps2 \<equiv>
    map_op (case_sum id id) (case_sum id id)
-   (comp_op [(map (\<lambda> p. Inr (0 :: 2, p)) enum_class.enum) [\<mapsto>] (map (\<lambda> p. Inr (1 :: 2, p)) enum_class.enum)] buf1 (inp_top os1 caps1 inps) (m_top os2 buf2 caps2))"
+   (comp_op [Inr (0 :: 2, 0 :: 1) \<mapsto> Inr (1 :: 2, 0 :: 1)] buf1 (inp_top os1 caps1 inps) (m_top os2 buf2 caps2))"
 
 
 (* FIXME: move me *)
@@ -219,25 +220,260 @@ lemma propagate_pointstamps_append:
 
 (* edges sg = (\<lambda> l. if node l = 0 \<and> port l = Src 1 then [Loc 1 (Trg 0)] else []) \<Longrightarrow> *)
 
+term "map (\<lambda> xs. case xs of [] \<Rightarrow> [] | xs \<Rightarrow> [Max (set xs)])"
+
+(* FIXME: move me *)
+lemma map_in_setD:
+  "map f xs = ys \<Longrightarrow>
+   x \<in> set xs \<Longrightarrow>
+   f x \<in> set ys"
+  by force
+
 lemma
-  \<open>input_invar (\<lambda> p. n p + length (xs1 p) + length (xs2 p)) xs3 (outpu os1) \<Longrightarrow>
-   input_invar (\<lambda> p. n p + length (xs1 p)) xs2 (map projr o buf1 o Inr o Pair 1) \<Longrightarrow>
-   dataflow_op sg (inp_m_top os1 (\<lambda> p. n p + length (xs1 p) + length (xs2 p) + length (xs3 p)) inps buf1 os2 buf2 caps2) \<approx>
-   map_op (\<lambda> p. (1, p)) (\<lambda> p. (1, p)) (max_op n (\<lambda> p. xs1 p @@- xs2 p @@- xs3 p @@- inps p))\<close>
-  term "outpu os1"
-  term buf2
-  term xs3
-  term "outpu os1"
-
-  term "\<lambda> c. case c of Cap t p \<Rightarrow> (buf2 )"
-
-proof (coinduction arbitrary: inps1 inps2 buf1 buf2 inrbufs1 xs ys i j sg rule: weakBisimWeakUptoBisim)
-  case SIM2
+  \<open>input_invar (\<lambda> p. n p + length (xs1 p) + length (xs2 p) + length (xs3 p)) xs4 (outpu os1) \<Longrightarrow>
+   input_invar (\<lambda> p. n p + length (xs1 p) + length (xs2 p)) xs3 (map projr o buf1 o Inr o Pair 1) \<Longrightarrow>
+   buf2l = fold (\<lambda> cap f. f(out cap := f (out cap) @ map (\<lambda> x. (x, time cap)) (buf2 cap))) caps2 (\<lambda> p. []) \<Longrightarrow>
+   input_invar (\<lambda> p. n p + length (xs1 p)) xs2 buf2l \<Longrightarrow>
+   input_invar n (\<lambda> p. map (\<lambda> xs. case xs of [] \<Rightarrow> [] | xs \<Rightarrow> [Max (set xs)]) (xs1 p)) (outpu os2) \<Longrightarrow>
+   dataflow_op sg (inp_m_top os1 (\<lambda> p. n p + length (xs1 p) + length (xs2 p) + length (xs3 p) + length (xs4 p)) inps buf1 os2 buf2 caps2) \<approx>
+   map_op (\<lambda> p. (1, p)) (\<lambda> p. (1, p)) (max_op n (\<lambda> p. xs1 p @@- xs2 p @@- xs3 p @@- xs4 p @@- inps p))\<close>
+proof (coinduction arbitrary: os1 os2 n caps2 xs1 xs2 xs3 xs4 buf1 buf2 buf2l inps  sg rule: weakBisimWeakUptoBisimCong)
+  case SIM1
   then show ?case
     apply -
     unfolding wsim_def
     apply safe
-    apply (elim step_max'_top_elim step_map_op_elim step_comp_op_elim step_dataflow_op_elim step_input_top_elim conjE; simp split: if_splits option.splits; hypsubst_thin)
+    apply (elim step_max'_top_elim step_map_op_elim step_comp_op_elim step_dataflow_op_elim step_input_top_elim conjE; simp split: if_splits option.splits add: map_upd_upds_conv_if; hypsubst_thin)
+    subgoal for io op1' nid op'' x io' op''a pa op2' io'a op''b xs
+      apply (cases x; hypsubst_thin)
+      apply (drule input_invar_elim[where buf="\<lambda>p. map (case_list [] (\<lambda>a list. [Max (insert a (set list))])) (xs1 1)"])
+       apply assumption
+      apply safe
+      apply (clarsimp simp add: map_eq_append_conv split: list.splits)
+      subgoal for l zs la zsa x xs'
+        apply (intro conjI exI)
+         apply (rule step_wstep)
+         apply (rule step_map_op)
+          apply (rule step_max_op_Out_intro2[where p=0])
+            apply (subst ldropWhile_lshift[where x="x # xs'"])
+              apply simp
+             apply simp
+            apply (subst dropWhile_append2)
+        subgoal premises prems for x
+          using prems(1,7,11) apply -
+          apply (drule map_in_setD)
+           apply assumption
+          apply (auto split: list.splits)
+          done
+            apply simp
+           apply simp
+          apply (simp add: defaults_num1_def)
+         apply simp
+         apply (subst ltakeWhile_lfshift[where x="x # xs'"])
+           apply simp
+          apply simp
+         apply simp
+         apply (subst takeWhile_append2)
+        subgoal premises prems for x
+          using prems(1,7,11) apply -
+          apply (drule map_in_setD)
+           apply assumption
+          apply (auto split: list.splits)
+          done
+         apply simp
+         apply (metis (no_types, lifting) length_map)
+        subgoal premises prems
+          apply (intro relcomppI)
+            apply (rule bisim_refl)
+           defer
+           apply (rule wbisim_refl)
+          apply simp
+          apply (rule wb_upto_b_base)
+          apply (rule exI[of _ os1])
+          apply (rule exI[of _ "os2\<lparr> outpu := (outpu os2)(1 := xs) \<rparr>"])
+          apply (intro exI conjI)
+               prefer 6
+          using prems(9) apply -
+                   apply (rule input_invar_cong)
+                  apply assumption
+                 apply (rule refl)+
+                defer
+          apply simp
+               apply (rule arg_cong2[where f=dataflow_op])
+                apply (rule refl)+
+               apply (rule arg_cong3[where f=map_op])
+                 apply simp_all
+               apply (rule arg_cong4[where f=comp_op])
+                  apply simp_all
+               apply (rule arg_cong3[where f=map_op])
+                 apply simp_all
+               apply (rule arg_cong3[where f=input_top])
+                 apply simp_all
+               apply (rule ext)
+               apply simp_all
+          defer
+               apply (rule arg_cong3[where f=map_op])
+                 apply simp_all
+               apply (rule arg_cong2[where f=max_op])
+               apply (rule ext)
+                apply simp_all
+               apply force
+              apply simp_all
+          prefer 5
+            apply (subst ltakeWhile_lfshift[where x="x # xs'"])
+                apply simp_all
+        apply (subst takeWhile_append2)
+        subgoal 
+          using prems apply -
+          apply (drule map_in_setD)
+           apply assumption
+          apply (auto split: list.splits)
+          done
+            apply simp
+        subgoal
+          using prems(3) apply -
+          apply (rule input_invar_cong)
+             apply assumption
+            apply simp_all
+           apply (rule ext)
+           apply auto
+        apply (subst ltakeWhile_lfshift[where x="x # xs'"])
+                apply simp_all
+        apply (subst takeWhile_append2)
+        subgoal 
+          using prems apply -
+          apply (drule map_in_setD)
+           apply assumption
+          apply (auto split: list.splits)
+          done
+        apply simp
+        done
+        subgoal
+          using prems(4) apply -
+ apply (rule input_invar_cong)
+             apply assumption
+            apply simp_all
+           apply (rule ext)
+           apply auto
+        apply (subst ltakeWhile_lfshift[where x="x # xs'"])
+                apply simp_all
+        apply (subst takeWhile_append2)
+        subgoal 
+          using prems apply -
+          apply (drule map_in_setD)
+           apply assumption
+          apply (auto split: list.splits)
+          done
+        apply simp
+        done
+      subgoal
+          using prems(5) apply -
+          apply (rule input_invar_cong)
+             apply assumption
+            apply simp_all
+           apply (rule ext)
+           apply auto
+        apply (subst ltakeWhile_lfshift[where x="x # xs'"])
+                apply simp_all
+        apply (subst takeWhile_append2)
+        subgoal 
+          using prems apply -
+          apply (drule map_in_setD)
+           apply assumption
+          apply (auto split: list.splits)
+          done
+        apply simp
+        done
+    subgoal
+          using prems(9,2) apply -
+         
+          find_theorems "concat _ = concat _"
+
+end
+          apply (rule exI[of _ os1])
+            apply (rule exI[of _ "os2\<lparr> outpu := (outpu os2)(1 := xs) \<rparr>"])
+            apply (rule exI[of _ "n(0 := Suc (dataflow_topology_from_tree.followed_by (n 0) (the_enat (llength (ltakeWhile ((=) []) ((la @ (x # xs') # zsa) @@- xs2 1 @@- xs3 1 @@- xs4 1 @@- inps 1))))))"])
+            apply (rule exI[of _ caps2])
+          apply (rule exI[of _ "xs1( 0 := zsa)"])
+          apply (rule exI[of _ "xs2"])
+          apply (rule exI[of _ "xs3"])
+          apply (rule exI[of _ "xs4"])
+            apply (rule exI[of _ "buf1"])
+            apply (rule exI[of _ "buf2"])
+          apply (rule exI[of _ "inps"])
+            apply (intro exI[of _ sg] conjI)
+                 apply (rule refl)+
+                 apply simp
+          subgoal
+               apply (rule input_invar_cong)
+          using prems(3) apply assumption 
+                 defer
+            apply (rule refl)+
+          apply (rule ext)
+          apply auto
+        apply (subst ltakeWhile_lfshift[where x="x # xs'"])
+            apply simp_all
+                   apply (subst takeWhile_append2)
+          using prems(1,7) apply -
+          using
+            \<open>\<And>xb. map (case_list [] (\<lambda>a list. [Max (insert a (set list))])) la = map fst l \<Longrightarrow> map (case_list [] (\<lambda>a list. [Max (insert a (set list))])) zsa = map fst zs \<Longrightarrow> input_invar (\<lambda>p. Suc (dataflow_topology_from_tree.followed_by (dataflow_topology_from_tree.followed_by (dataflow_topology_from_tree.followed_by (n 1) (dataflow_topology_from_tree.followed_by (length la) (length zsa))) (length (xs2 1))) (length (xs3 1)))) xs4 (outpu os1) \<Longrightarrow> input_invar (\<lambda>p. Suc (dataflow_topology_from_tree.followed_by (dataflow_topology_from_tree.followed_by (n 1) (dataflow_topology_from_tree.followed_by (length la) (length zsa))) (length (xs2 1)))) xs3 ((map projr \<circ> buf1 \<circ> Inr \<circ>\<circ> Pair) 1) \<Longrightarrow> input_invar (\<lambda>p. Suc (dataflow_topology_from_tree.followed_by (n 1) (dataflow_topology_from_tree.followed_by (length la) (length zsa)))) xs2 (fold (\<lambda>cap f. f(1 := f 1 @ map (\<lambda>x. (x, time cap)) (buf2 cap))) caps2 (\<lambda>p. [])) \<Longrightarrow> outpu os2 1 = (Max (insert x (set xs')), dataflow_topology_from_tree.followed_by (n 1) (length l)) # xs \<Longrightarrow> \<forall>x\<in>set l. fst x = [] \<Longrightarrow> [n 1..< dataflow_topology_from_tree.followed_by (n 1) (dataflow_topology_from_tree.followed_by (length la) (length zsa))] @ [dataflow_topology_from_tree.followed_by (n 1) (dataflow_topology_from_tree.followed_by (length la) (length zsa))] = map snd l @ dataflow_topology_from_tree.followed_by (n 1) (length l) # map snd zs \<Longrightarrow> input_invar (n(1 := dataflow_topology_from_tree.followed_by (n 1) (length l))) ((\<lambda>p. map fst l @ [Max (insert x (set xs'))] # map fst zs) (1 := [] # map fst zs)) ((outpu os2)(1 := xs)) \<Longrightarrow> xs1 1 = la @ (x # xs') # zsa \<Longrightarrow> xb \<in> set la \<Longrightarrow> [] = xb\<close>
+            prems(10,2,3,4,5,6,8,9) apply blast
+          apply simp
+          done
+        subgoal
+               apply (rule input_invar_cong)
+          using prems(4) apply assumption 
+          apply (rule ext)
+          apply auto
+  apply (subst ltakeWhile_lfshift[where x="x # xs'"])
+            apply simp_all
+                   apply (subst takeWhile_append2)
+          using prems(1,7) apply -
+          using
+            \<open>\<And>xb. map (case_list [] (\<lambda>a list. [Max (insert a (set list))])) la = map fst l \<Longrightarrow> map (case_list [] (\<lambda>a list. [Max (insert a (set list))])) zsa = map fst zs \<Longrightarrow> input_invar (\<lambda>p. Suc (dataflow_topology_from_tree.followed_by (dataflow_topology_from_tree.followed_by (dataflow_topology_from_tree.followed_by (n 1) (dataflow_topology_from_tree.followed_by (length la) (length zsa))) (length (xs2 1))) (length (xs3 1)))) xs4 (outpu os1) \<Longrightarrow> input_invar (\<lambda>p. Suc (dataflow_topology_from_tree.followed_by (dataflow_topology_from_tree.followed_by (n 1) (dataflow_topology_from_tree.followed_by (length la) (length zsa))) (length (xs2 1)))) xs3 ((map projr \<circ> buf1 \<circ> Inr \<circ>\<circ> Pair) 1) \<Longrightarrow> input_invar (\<lambda>p. Suc (dataflow_topology_from_tree.followed_by (n 1) (dataflow_topology_from_tree.followed_by (length la) (length zsa)))) xs2 (fold (\<lambda>cap f. f(1 := f 1 @ map (\<lambda>x. (x, time cap)) (buf2 cap))) caps2 (\<lambda>p. [])) \<Longrightarrow> outpu os2 1 = (Max (insert x (set xs')), dataflow_topology_from_tree.followed_by (n 1) (length l)) # xs \<Longrightarrow> \<forall>x\<in>set l. fst x = [] \<Longrightarrow> [n 1..< dataflow_topology_from_tree.followed_by (n 1) (dataflow_topology_from_tree.followed_by (length la) (length zsa))] @ [dataflow_topology_from_tree.followed_by (n 1) (dataflow_topology_from_tree.followed_by (length la) (length zsa))] = map snd l @ dataflow_topology_from_tree.followed_by (n 1) (length l) # map snd zs \<Longrightarrow> input_invar (n(1 := dataflow_topology_from_tree.followed_by (n 1) (length l))) ((\<lambda>p. map fst l @ [Max (insert x (set xs'))] # map fst zs) (1 := [] # map fst zs)) ((outpu os2)(1 := xs)) \<Longrightarrow> xs1 1 = la @ (x # xs') # zsa \<Longrightarrow> xb \<in> set la \<Longrightarrow> [] = xb\<close>
+            prems(10,2,3,4,5,6,8,9) apply blast
+          apply simp
+          done
+           apply simp_all
+        prefer 3
+        subgoal
+          apply (rule wbisim_map_op)
+          apply (rule wbisim_refl_alt)
+          apply (rule arg_cong2[where f=max_op])
+           apply auto
+          apply (rule ext)
+          apply auto
+
+        find_theorems map_op wbisim
+
+
+        find_theorems input_invar
+
+end
+                apply (rule wb_upto_b_base)
+                defer
+                apply (rule wbisim_refl)
+               apply (rule bisim_refl)
+
+
+          find_theorems takeWhile append
+
+         thm map_eq_append_conv
+
+end
+             apply force
+            apply simp
+           apply simp
+          apply (simp add: defaults_num1_def)
+         apply simp
+         apply (intro conjI)
+        
+
+      thm input_invar_elim
+
+      find_theorems  defaults 
+
+
     defer
   (*   subgoal for op'' io' op''a p op1' q io'a op''b xa xs
       apply (cases inps1; simp)
